{
 "cells": [
  {
   "cell_type": "markdown",
   "id": "6fa3b6ff",
   "metadata": {},
   "source": [
    "$\\textbf{PROGRAMMING ASSIGNMENTS (PRE-MIDTERMS)}$"
   ]
  },
  {
   "cell_type": "markdown",
   "id": "dc3a9079-43d4-441c-a672-948cca075ecf",
   "metadata": {},
   "source": [
    "$\\textbf{Assignment}$ instructions:\n",
    "- Use latex.\n",
    "- Write your latex in jupyter notebook.\n",
    "- Push your answers to your github account.\n",
    "- Deadline is 2 weeks before finals.\n",
    "- Fail to submit 2 weeks before finals is an automatic 5.0 for this assignment.\n",
    "- Each problem is 25 points.\n"
   ]
  },
  {
   "cell_type": "markdown",
   "id": "170c013d-2fc9-4f79-827e-fa9c95a6ad52",
   "metadata": {},
   "source": [
    "$\\textbf{Answers:}$"
   ]
  },
  {
   "cell_type": "markdown",
   "id": "07fb964f-80f3-4fda-9ae5-311d8fba0f7b",
   "metadata": {},
   "source": [
    "1. Recall the definition of a rational number, denoted as $\\mathbb{Q}$. Prove that the Euler's number $e = \\Sigma_{k=0}^\\infty \\frac{1}{k!} \\notin \\mathbb{Q}$. A factorial is defined as $k! = (k)(k-1)(k-2)(k-3)..., \\forall k \\in \\mathbb{Z}^+$, note that $0! = 1$. Furthermore, a sum notation $\\Sigma_{k=0}^\\infty k = 0+ 1 + 2 + 3 +....+...$\n",
    "\n",
    "    Step 1: Suppose $e$ is rational such that...\n",
    "\n",
    "    $e = \\frac{p}{q} = \\Sigma_{k=0}^\\infty \\frac{1}{k!}$\n",
    "\n",
    "    Where $p$ and $q$ are integers with no common factors other than 1.\n",
    "\n",
    "    Step 2: Let's consider the series of expansion of $e$:\n",
    "\n",
    "    $e = \\frac{p}{q} = \\Sigma_{k=0}^\\infty \\frac{1}{k!} = 1 + \\frac{1}{1!} + \\frac{1}{2!} + \\frac{1}{3!} + ...$\n",
    "\n",
    "    If $e$ is rational, then this infinite series must also be a rational number.\n",
    "\n",
    "    Step 3: Let's denote the partial sum of the series up to some integer $n$ as $S_n$:\n",
    "\n",
    "    $S_n = 1 + \\frac{1}{1!} + \\frac{1}{2!} +...+ \\frac{1}{n!}$\n",
    "\n",
    "    Step 4: Consider the difference between consecutive partial sums.\n",
    "\n",
    "    $S_n+1 - S_n = (1 + \\frac{1}{1!} + \\frac{1}{2!} +...+ \\frac{1}{n!}) - (1 + \\frac{1}{1!} + \\frac{1}{2!} +...+ \\frac{1}{n!} + \\frac{1}{n+1}!)$\n",
    "\n",
    "    $=\\frac{1}{n+1}!$\n",
    "\n",
    "    Each term in this difference is a positive fraction. So, $S_n+1$ is always greater than $S_n$, meaning partial sums are increasing. However, $e$ is defined as the limit of this sequence of partial sums as $n$ approaches infinity. If $e$ were rational, this sequence of partial sums would converge to a rational number. But since the sequence is always increasing, it cannot converge to a rational number.\n",
    "\n",
    "    Hence, Euler's number $e$ cannot be rational."
   ]
  },
  {
   "cell_type": "markdown",
   "id": "1730e23a-9c1b-40db-ae12-d19ef8a2ce33",
   "metadata": {},
   "source": [
    "2. Prove Minkowski's Inequality for sums, $\\forall \\ p>1, (a_k, b_k)>0$:\n",
    "\\begin{gather}\n",
    "\\left( \\sum_{k=1}^n |a_k + b_k|^p \\right)^{1/p} \\leq \\left( \\sum_{k=1}^n |a_k|^p \\right)^{1/p} + \\left( \\sum_{k=1}^n |b_k|^p \\right)^{1/p}\n",
    "\\end{gather}\n",
    "\n",
    "    Step 1: Minkowski's inequality states that for $( p > 1)$ and sequences of real numbers $(a_k)$ and $(b_k)$, the following inequality holds:\n",
    "   \n",
    "    $(\\Sigma_{k=1}^n | a_k + b_k |^p)^\\frac{1}{p} \\leq (\\Sigma_{k=1}^n | a_k | ^p)^\\frac{1}{p} + (\\Sigma_{k=1}^n | a_k | ^p)^\\frac{1}{p}$\n",
    "\n",
    "    To prove Minkowski;s inequality, we'll use Hölder's inequality. Hölder's inequality states that for any $p>1$, q such that $\\frac{1}{p} + \\frac{1}{q} = 1$, and sequences $(x_k)$ and $(y_k)$ of real numbers, the follwing inequality holds:\n",
    "\n",
    "   $\\Sigma_{k=1}^n | x_k y_k | \\leq (\\Sigma_{k=1}^n | x_k | ^p)^\\frac{1}{p}(\\Sigma_{k=1}^n | y_k | ^p)^\\frac{1}{q}$\n",
    "\n",
    "   Step 2: Now we choose sequences $(x_k)$ and $(y_k)$ that allows us to apply Hölder's inequality to obtain Minkowski's inequality, we define:\n",
    "\n",
    "   Let $x_k = \\frac{|a_k|}{(\\Sigma_{k=1}^n | a_k | ^p)^\\frac{1}{p}}$ and $y_k = \\frac{|b_k|}{(\\Sigma_{k=1}^n | b_k | ^p)^\\frac{1}{p}}$\n",
    "\n",
    "   These sequences are chosen such that Hölder's inequality is applied, it simplifies to Minkowski's inequality.\n",
    "\n",
    "   Step 3: Then, apply Hölder's inequality with $p$ and $q$ such that $\\frac{1}{p}+\\frac{1}{q}=1$, we substitute the sequence $(x_k)$ and $(y_k)$ into Hölder's inequality. By doing so, we obtain an inequality involving the absolute values of $a_k$ and $b_k$.\n",
    "\n",
    "$$\n",
    "\\sum_{k=1}^n \\frac{|a_k|}{\\left(\\sum_{k=1}^n |a_k|^p\\right)^{1/p}} \\cdot \\frac{|b_k|}{\\left(\\sum_{k=1}^n |b_k|^q\\right)^{1/q}} \\leq \\left(\\sum_{k=1}^n \\left(\\frac{|a_k|}{\\left(\\sum_{k=1}^n |a_k|^p\\right)^{1/p}}\\right)^p\\right)^{1/p} \\left(\\sum_{k=1}^n \\left(\\frac{|b_k|}{\\left(\\sum_{k=1}^n |b_k|^q\\right)^{1/q}}\\right)^q\\right)^{1/q}\n",
    "$$\n",
    "\n",
    "   $= (\\Sigma_{k=1}^n \\frac{|a_k|^p}{\\Sigma_{k=1}^n |a_k|^p})^\\frac{1}{p} (\\Sigma_{k=1}^n \\frac{|b_k|^p}{\\Sigma_{k=1}^n |b_k|^p})^\\frac{1}{q}$\n",
    "\n",
    "   $=1.1=1$\n",
    "\n",
    "    So, we have:\n",
    "\n",
    "   $\\Sigma_{k=1}^n \\frac{|a_k b_k|}{(\\Sigma_{k=1}^n |a_k|^p)^\\frac{1}{p}(\\Sigma_{k=1}^n |b_k|^p)^\\frac{1}{p})} \\leq 1$\n",
    "\n",
    "   Step 4: Then, we take both sides of the inequality to the power of $p$. This is a common step in proofs involving inequalities, as it often simplifies expressions and allows for easier manipulation.\n",
    "\n",
    "   $(\\Sigma_{k=1}^n |a_k b_k|^p)^\\frac{1}{p} \\leq(\\Sigma_{k=1}^n |a_k|^p)^\\frac{1}{p} (\\Sigma_{k=1}^n |b_k|^p)^\\frac{1}{p}$\n",
    "\n",
    "   After taking powers, we rearrange the terms to isolate the sum of $\\Sigma_{k=1}^n |a_k b_k|^p$.\n",
    "\n",
    "   Step 5: Finally, we take both sides of the inequality of the inequality to the power of $\\frac{1}{p}$, which effectively taking $pth$ root of both sides. This yields Minkowski's inequality in its standard form.\n",
    "\n",
    "   $(\\Sigma_{k=1}^n |a_k + b_k|^p)^\\frac{1}{p} \\leq (\\Sigma_{k=1}^n |a_k|^p)^\\frac{1}{p} + (\\Sigma_{k=1}^n |b_k|^p)^\\frac{1}{p}$\n",
    "\n",
    "   $\\textbf{Hence, we have proven Minkowski's inequality for sums, which states that for $p>1$ and sequences $(a_k)$ $(b_k)$ of positive real numbers.}$"
   ]
  },
  {
   "cell_type": "markdown",
   "id": "65494c64-414d-4d3a-8528-1f69ada0ed45",
   "metadata": {},
   "source": [
    "3. Prove the triangle inequality $|x+y| \\leq |x| + |y|, \\forall (x,y) \\in \\mathbb{R}$\n",
    "\n",
    "   To prove the traingle inequality $|x+y| \\leq |x|+|y|$ for all real numbers $x$ and $y$, we'll consider two cases:\n",
    "\n",
    "    - Both $x$ and $y$ are non-negative.\n",
    "    - Atleast one of $x$ and $y$ is negative.\n",
    "\n",
    "     Case 1: Both $x$ and $y$ are non-negative.\n",
    "\n",
    "    - In this case, both $x$ and $y$ are non-negative, so their absolute values are just themselves, $|x| = x$ and $|y| = y$.\n",
    "    - The expression $|x+y|$ represents the absolute value of the sum $x+y$, which is the same as the sum itself when both $x$ and $y$ are non-negative.\n",
    "  \n",
    "      Hence, in this case, the inequality $|x+y| = |x| + |y|$ is satisfied, affirming the validity of the triangle in inequality for non-negative real numbers $x$ and $y$.\n",
    "\n",
    "   Case 2: Atleast one of $x$ and $y$ is negative.\n",
    "\n",
    "      - Here, we consider the scenario where either $x$ or $y$ or both is/are negative. Without loss of generality, we assume $x \\geq 0$ $x < 0$.\n",
    "      - The absolute value of $x+y$ is $x-y$, because y is negative and when we subtract a negative number, its like adding its absolute value.\n",
    "      - Similarly, the sum of $|x|$ and $|y|$ is $x-y$, because the absolute value of $y$ is its negative counter part $-y$, and when we add a negative number its like subtracting its absolute value.\n",
    "  \n",
    "        Hence, in both cases, we've shown that $|x+y|$ is less than or equal to $|x| + |y|$, which confirms the triangle inequality for all realy numers $x$ and $y$."
   ]
  },
  {
   "cell_type": "markdown",
   "id": "b1cb9273-676b-4cdb-894f-d6c3727d2906",
   "metadata": {},
   "source": [
    "4. Prove Sedrakayan's Lemma $\\forall u_i, v_i \\in \\mathbb{R}^+$:\n",
    "\\begin{gather}\n",
    "\\frac{(\\Sigma_{i=1}^n u_i)^2}{\\Sigma_{i=1}^n v_i}\n",
    "\\leq\n",
    "\\Sigma_{i=1}^n \\frac{(u_i)^2}{v_i}\n",
    "\\end{gather}\n",
    "\n",
    "    Step 1: To prove Sedrakayan's Lemma, we use the Cauchy-Schwarz inequality. The Cauchy-Schwarz inquality states:\n",
    "\n",
    "    $(\\Sigma_{i=1}^n a_i b_i)^2 \\leq (\\Sigma_{i=1}^n a^2_i) (\\Sigma_{i=1}^n b^2_i)$\n",
    "\n",
    "   Step 2: We substitute back by denoting $a_i = \\sqrt{u_i}$ and $b_i = \\sqrt{v_i}$. This is a common technique used to simplify expressions involving square roots. So, we get:\n",
    "\n",
    "   $(\\Sigma_{i=1}^n  \\sqrt{u_i} \\sqrt{v_i})^2 \\leq (\\Sigma_{i=1}^n u_i) (\\Sigma_{i=1}^n v_i)$\n",
    "\n",
    "   Now we gave substituted $a_i = \\sqrt{u_i}$ and $b_i = \\sqrt{v_i}$ into the Cauchy-Schwarz inequality.\n",
    "\n",
    "   Step 3: We square both sides of the inequality obtained from the Cauchy-Schwarz inequality. This is a valid step since both sides of the inequality are non-negative.\n",
    "\n",
    "   $(\\Sigma_{i=1}^n u_i v_i)^2 \\leq (\\Sigma_{i=1}^n u_i) (\\Sigma_{i=1}^n v_i)^2$\n",
    "\n",
    "    Step 4: We divide both sides of the squared inequality by $(\\Sigma_{i=1}^n u_i)^2$. Because we are diving by a positive quantity. Since all $u_i$ are positive, as given in the lemma statement.\n",
    "\n",
    "   $\\frac{(\\Sigma_{i=1}^n u_i)}{\\Sigma_{i=1}^n v_i} \\leq \\Sigma_{i=1}^n \\frac{(u_i)^2}{v_i}$\n",
    "\n",
    "   Hence, we have proved that the square of the sum of $u_i$ divided by the sum of $v_i$ is less than or equal to the sum of the squares of $u_i/v_i$ for $i$ from 1 to $n$."
   ]
  },
  {
   "cell_type": "markdown",
   "id": "73c09dd3-c66b-43a4-bad8-836b1bf1313c",
   "metadata": {},
   "source": [
    "1. Consider the functions $f(x) = 2x+1$, $g(x)=2y-1$, $j(x) = |f(x)+g(x)|$, and $h(x) = j(x)^2$, show for the following inequality that:\n",
    "\n",
    "\\begin{gather}\n",
    "\\sqrt{|f(x)|^2} \\geq \\sqrt{h(x)} - \\sqrt{|g(x)|^2}, \\forall (x,y) \\in \\mathbb{Z}^+\n",
    "\\end{gather}\n",
    "\n",
    "Step 1: We rewrite the absolute functions $|f(x)|$ and $|g(x)|$ using the definition of absolute value.\n",
    "\n",
    "$|f(x)| = |2x+1|$\n",
    "\n",
    "$|g(x)| = |2y-1|$\n",
    "\n",
    "Step 2: We simplify the left-hand side. We know that for any real numbers $a$, $\\sqrt{a^2} = |a|$. So, we can rewrite the left-hand side of the given inequalities as:\n",
    "\n",
    "$\\sqrt{|f(x)|^2} = |f(x)|$\n",
    "\n",
    "Step 3: We rewrite $h(x)$ in terms of $j(x)$. Since $h(x) = j(x)^2$.\n",
    "\n",
    "$h(x) = j(x)^2 = (|f(x)| + g(x))^2$\n",
    "\n",
    "Step 5: We subsitute the expression j(x) into the h(x), so...\n",
    "\n",
    "$h(x) = (|f(x)| + |g(x)|)$\n",
    "\n",
    "Now our inequality becomes: $|f(x)| \\geq \\sqrt{h(x)} - g(x)$\n",
    "\n",
    "Step 6: We substitute the expressions for $|f(x)|$ and $|g(x)|$ back into the inequality, simplifying it step by step.\n",
    "\n",
    "$|2x+1| \\geq \\sqrt{j(x)^2} - |2y-1|$\n",
    "\n",
    "Step 7: We expand the absolute value expressions and simplify to get $|2x+1|$,$|2x+2y|$, and $|2y-1|$. Because give that $j(x) = |f(x) + g(x)|$, we can simplify it further:\n",
    "\n",
    "$2x+1 \\geq \\sqrt{|f(x) + g(x)|^2} - |2y-1|$\n",
    "\n",
    "$2x+1 \\geq |f(x) + g(x)| - |2y-1|$\n",
    "\n",
    "$2x+1 \\geq |(2x+1) + (2y-1) - |2y-1|$\n",
    "\n",
    "$2x+1 \\geq |2x + 2y| - |2y-1|$\n",
    "\n",
    "Step 8: Finally, we verify the inequality for two cases: when 2x+1 is positive and when its negative. In each case, we substitute the expressions for $|f(x)|$, $|2x + 2y|$, and $|2y-1|$. We simplify to check if the inequality holds true. If it holds true for both cases, then it proves that the inequality holds true for all positive integers $x$ and $y$.\n",
    "\n",
    "Case 1: When $2x+1$ is positive.\n",
    "\n",
    "$|2x+1| = 2x+1$\n",
    "\n",
    "$|2x+2y| = 2x+2y$\n",
    "\n",
    "$|2y-1| = 2y-1$\n",
    "\n",
    "The inequality becomes:\n",
    "\n",
    "$2x+1 \\geq (2x+2y)-(2y-1)$\n",
    "\n",
    "$2x+1 \\geq 2x+2y - 2y+1$\n",
    "\n",
    "$2x+1 \\geq 2x+1$\n",
    "\n",
    "This case holds true for all positive integers $x$ and $y$ when $2x+1$ is positive.\n",
    "\n",
    "Case 2: When $2x+1$ is negative.\n",
    "\n",
    "$|2x+1| = -(2x+1)$\n",
    "\n",
    "$|2x+2y| = -(2x+2y)$\n",
    "\n",
    "$|2y-1| = 2y-1$\n",
    "\n",
    "The inequality becomes: \n",
    "\n",
    "$-(2x+1) \\geq -(2x+2y)-(2y-1)$\n",
    "\n",
    "$-2x+1 \\geq -2x-2y-2y+1$\n",
    "\n",
    "$-2x+1 \\geq -2x-4y+1$\n",
    "\n",
    "This case also holds true for all positive integers $x$ and $y$ when $2x+1$ is negative.\n",
    "\n",
    "Hence, the inequality holds true for all positive integers $x$ and $y$."
   ]
  },
  {
   "cell_type": "markdown",
   "id": "4166ba21-aff8-467a-864d-9501390c22d2",
   "metadata": {},
   "source": [
    "2. Prove Sedrakayan's Lemma if $u_i, v_i$ are square roots of an even integers:\n",
    "\\begin{gather}\n",
    "\\frac{(\\Sigma_{i=1}^n u_i)^2}{\\Sigma_{i=1}^n v_i}\n",
    "\\leq\n",
    "\\Sigma_{i=1}^n \\frac{(u_i)^2}{v_i}\n",
    "\\end{gather}\n",
    "\n",
    "    We are given that $u_i$ and $v_i$ are square roots of even integers.\n",
    "\n",
    "   Step 1: We denote $A$ as the sum of all $u_i$ and B as the sum of all $v_i$.\n",
    "\n",
    "   $A = \\Sigma_{i=1}^n u_i$\n",
    "   \n",
    "   $B = \\Sigma_{i=1}^n v_i$\n",
    "\n",
    "   Step 2: We need to prove that:\n",
    "\n",
    "   $\\frac{A^2}{B} \\leq \\Sigma_{i=1}^n \\frac{(u_i)^2}{v_i}$\n",
    "\n",
    "   Step 3: We expand $\\frac{A^2}{B}$, using the definition of $A$ and $B$. We substitute them into the expression.\n",
    "\n",
    "   $\\frac{A^2}{B} = \\frac{(\\Sigma_{i=1}^n u_i)^2}{\\Sigma_{i=1}^n v_i}$\n",
    "\n",
    "   $= \\frac{\\Sigma_{i=1}^n u_i . \\Sigma_{j=1}^n u_j}{\\Sigma_{k=1}^n v_k}$\n",
    "\n",
    "   Step 4: We expand $\\Sigma_{i=1}^n \\frac{(u_i)^2}{v_i}$ by writing out each term seperately.\n",
    "\n",
    "    $\\Sigma_{i=1}^n \\frac{(u_i)^2}{v_i} = \\frac{(u_1)^2}{v_1} + \\frac{(u_2)^2}{v_2} +...+\\frac{(u_n)^2}{v_n}$\n",
    "\n",
    "   Step 5: We observe that $u_i$ and $v_i$ are square roots of integers, their $u_i^2$ and $v_i$ are integers.\n",
    "\n",
    "   Step 6: Finally, we apply the Cauch-Schwarz inequality, which stat for any real numbers $a_1$, $a_2$, $...a_n$ and $b_1$,$b_2$,$...b_n$, the following holds:\n",
    "\n",
    "   $(\\Sigma_{i=1}^n a_i . b_i)^2 \\leq (\\Sigma_{i=1}^n a_i^2) . (\\Sigma_{i=1}^n b_i^2)$\n",
    "\n",
    "  Hence, by Cauchy-Schwarz inequality, this shows that $\\frac{A^2}{B}$ is indeed less than or equal to $\\Sigma_{i=1}^n \\frac{(u_i)^2}{v_i}$\n",
    "\n",
    "   $\\frac{\\Sigma_{i=1}^n u_i . \\Sigma_{j=1}^n u_j}{\\Sigma_{k=1}^n v_k} \\leq \\Sigma_{i=1}^n \\frac{(u_i)^2}{v_i}$"
   ]
  }
 ],
 "metadata": {
  "kernelspec": {
   "display_name": "Python 3 (ipykernel)",
   "language": "python",
   "name": "python3"
  },
  "language_info": {
   "codemirror_mode": {
    "name": "ipython",
    "version": 3
   },
   "file_extension": ".py",
   "mimetype": "text/x-python",
   "name": "python",
   "nbconvert_exporter": "python",
   "pygments_lexer": "ipython3",
   "version": "3.12.3"
  }
 },
 "nbformat": 4,
 "nbformat_minor": 5
}
